src/goose_lang/lib/waitgroup/waitgroup.v
@@ -36,12 +36,16 @@ Local Coercion Var' (s:string): expr := Var s.
  *)
 
 Section proof.
-  Context `{!heapGS Σ} (N : namespace).
 
   Class waitgroupG Σ := {
       wg_tokG :> mapG Σ u64 unit;
       wg_totalG :> ghost_varG Σ u64 (* TODO: this will need to be mnat *)
   }.
+  Definition waitgroupΣ := #[mapΣ u64 unit ; ghost_varΣ u64].
+  Global Instance subG_waitgroupΣ {Σ} : subG (waitgroupΣ) Σ → (waitgroupG Σ).
+  Proof. solve_inG. Qed.
+
+  Context `{!heapGS Σ} (N : namespace).
   Context `{!waitgroupG Σ}.
 
   Record waitgroup_names :=
