src/program_proof/simplepb/pb_init_proof.v
@@ -4,6 +4,7 @@ From Goose.github_com.mit_pdos.gokv.simplepb Require Export pb.
 From Perennial.program_proof.simplepb Require Export pb_ghost.
 From Perennial.program_proof.simplepb Require Import pb_definitions.
 From Perennial.program_proof.grove_shared Require Import urpc_spec.
+From iris.algebra Require Import mono_list.
 
 Section pb_init_proof.
 
@@ -53,6 +54,37 @@ Proof.
   iExactEq "H1".
   f_equal.
   set_solver.
+Qed.
+
+Lemma pb_init_log γsys :
+  own_ghost γsys [] ={⊤}=∗
+  ∃ γlog, own_log γlog [] ∗ is_inv γlog γsys
+.
+Proof.
+  iIntros "Hghost".
+  iMod (own_alloc (●ML [])) as (γlog) "[Hlog1 Hlog2]".
+  { apply mono_list_auth_valid. }
+  iExists _; iFrame "Hlog2".
+  iMod (inv_alloc with "[-]") as "$"; last done.
+  iNext.
+  iExists [].
+  iFrame.
+  iSplitL.
+  {
+    iExists [].
+    iFrame.
+    iSplitR; first done.
+    iApply big_sepL2_nil.
+    done.
+  }
+  iModIntro.
+  iIntros.
+  exfalso.
+  rewrite H0 in H.
+  apply prefix_nil_inv in H.
+  apply (f_equal length) in H.
+  rewrite app_length /= in H.
+  lia.
 Qed.
 
 End pb_init_proof.
